COMP/PCF_rep.v
@@ -12,14 +12,14 @@ Unset Strict Implicit.
 Unset Transparent Obligations.
 Unset Automatic Introduction.
 
-Notation "'TY'" := PCF.types.
+Notation "'TY'" := PCF.Sorts.
 Notation "'Bool'":= PCF.Bool.
 Notation "'Nat'":= PCF.Nat.
 
 Section rep.
 
 Notation "'IT'" := (ITYPE TY).
-Notation "a '~>' b" := (PCF.arrow a b) 
+Notation "a '~>' b" := (PCF.Arrow a b) 
      (at level 69, right associativity).
 Notation "a 'x' b" := (product (*C:= MOD _ _*) a b) (at level 30).
 Notation "P [ z ]" := (ITFIB_MOD _ z P) (at level 35).
