PCF/PCF_Monad.v
@@ -6,6 +6,47 @@ Unset Strict Implicit.
 Unset Transparent Obligations.
 Unset Automatic Introduction.
 
+
+Section close_notation.
+Notation "'TY'" := PCF.Sorts.
+Notation "'Bool'" := PCF.Bool.
+Notation "'Nat'" := PCF.Nat.
+
+Notation "'IT'" := (ITYPE TY).
+Notation "a '~>' b" := (PCF.Arrow a b) 
+   (at level 69, right associativity).
+Notation "M [*:= N ]" := (substar N M) (at level 50).
+Notation "'$' f" := (@_shift _ _ _ f) (at level 30).
+Notation "y >>- f" := (_shift f y) (at level 44).
+Notation "y >>= f" := (@subst _ _ f _ y) (at level 42).
+
+Notation "v //- f" := (@rename _ _ f _ v)(at level 43, left associativity).
+Ltac opt := simpl; intros; elim_opt.
+
+Ltac fin := simpl in *; intros; 
+   autorewrite with fin; auto with fin; simpl;
+	try reflexivity.
+Hint Unfold lift : fin.
+Hint Extern 1 (_ = _) => f_equal : fin.
+Hint Resolve rename_eq : fin.
+Hint Rewrite rename_eq : fin.
+Hint Resolve  rename_id shift_eq : fin.
+Hint Rewrite  rename_id shift_eq : fin.
+Hint Resolve shift_var : fin.
+Hint Rewrite shift_var : fin.
+Hint Resolve var_lift_shift_eq : fin.
+Hint Resolve shift_lift : fin.
+Hint Rewrite shift_lift : fin.
+Hint Resolve subst_eq : fin.
+Hint Rewrite subst_eq : fin.
+Hint Rewrite subst_rename rename_subst : fin.
+Hint Unfold inj : fin.
+Hint Resolve subst_shift_shift subst_var subst_var_eta : fin.
+Hint Rewrite subst_shift_shift subst_var subst_var_eta : fin.
+Hint Resolve subst_var subst_subst : fin.
+Hint Rewrite subst_subst : fin.
+Hint Rewrite lift_rename : fin.
+
 Obligation Tactic := fin.
 
 Program Instance PCFm : 
@@ -44,10 +85,11 @@ Qed.
 
 Hint Resolve shift_shift rename_lift : fin.
 Hint Rewrite shift_shift rename_lift : fin.
-
+(*
 Notation "'IT'" := (ITYPE TY).
 Notation "a '~>' b" := (PCF.arrow a b) 
      (at level 69, right associativity).
+*)
 Notation "a 'x' b" := (product a b) (at level 30).
 Notation "P [ z ]" := (ITFIB_MOD _ z P) (at level 35).
 Notation "'d' P // s" := (ITDER_MOD _ _ s P) (at level 25).
@@ -135,7 +177,7 @@ Program Instance bottom_hom_s t : Module_Hom_struct
 
 Canonical Structure PCFBottom t := Build_Module_Hom (bottom_hom_s t).
 
-
+End close_notation.
 
 
 
