PCF/PCF_RMonad.v
@@ -7,6 +7,44 @@ Unset Strict Implicit.
 Unset Transparent Obligations.
 Unset Automatic Introduction.
 
+Section close_notation.
+Notation "'TY'" := PCF.Sorts.
+Notation "'Bool'" := PCF.Bool.
+Notation "'Nat'" := PCF.Nat.
+
+Notation "'IT'" := (ITYPE TY).
+Notation "a '~>' b" := (PCF.Arrow a b) 
+   (at level 69, right associativity).
+Notation "M [*:= N ]" := (substar N M) (at level 50).
+Notation "'$' f" := (@_shift _ _ _ f) (at level 30).
+Notation "y >>- f" := (_shift f y) (at level 44).
+Notation "y >>= f" := (@subst _ _ f _ y) (at level 42).
+
+Ltac opt := simpl; intros; elim_opt.
+
+Ltac fin := simpl in *; intros; 
+   autorewrite with fin; auto with fin; simpl;
+	try reflexivity.
+Hint Unfold lift : fin.
+Hint Extern 1 (_ = _) => f_equal : fin.
+Hint Resolve rename_eq : fin.
+Hint Rewrite rename_eq : fin.
+Hint Resolve  rename_id shift_eq : fin.
+Hint Rewrite  rename_id shift_eq : fin.
+Hint Resolve shift_var : fin.
+Hint Rewrite shift_var : fin.
+Hint Resolve var_lift_shift_eq : fin.
+Hint Resolve shift_lift : fin.
+Hint Rewrite shift_lift : fin.
+Hint Resolve subst_eq : fin.
+Hint Rewrite subst_eq : fin.
+Hint Rewrite subst_rename rename_subst : fin.
+Hint Unfold inj : fin.
+Hint Resolve subst_shift_shift subst_var subst_var_eta : fin.
+Hint Rewrite subst_shift_shift subst_var subst_var_eta : fin.
+Hint Resolve subst_var subst_subst : fin.
+Hint Rewrite subst_subst : fin.
+Hint Rewrite lift_rename : fin.
 Obligation Tactic := fin.
 
 Program Instance PCFEM_s : RMonad_struct (IDelta TY) PCFE := {
@@ -36,7 +74,7 @@ Qed.
 
 
 Program Instance PCFApp_car_s :
-forall (r s : PCF.types) (c : TY -> Type),
+forall (r s : TY) (c : TY -> Type),
 PO_mor_struct (a:=PO_product (ipo_proj (PCFE c) (r ~> s)) 
                              (ipo_proj (PCFE c) r))
   (b:=ipo_proj (PCFE c) s)
@@ -65,7 +103,7 @@ Definition PCFApp_car r s:
 := fun c => Build_PO_mor (PCFApp_car_s r s c).
 
 Program Instance PCFApp_s:
-forall r s : PCF.types,
+forall r s : TY,
 RModule_Hom_struct
   (M:=Prod_RMod (P:=PCFEM) PO_prod 
        (Fib_RMod (P:=PCFEM) (r ~> s) PCFEM)
@@ -77,7 +115,7 @@ Notation "M [ z ]" := (FIB_RMOD _ z M) (at level 35).
 Notation "'d' M // s" := (DER_RMOD _ _ s M) (at level 25).
 Notation "a 'x' b" := (product a b) (at level 30).
 
-Definition PCFApp: forall r s : PCF.types, 
+Definition PCFApp: forall r s : TY, 
  (PCFEM [r ~> s]) x (PCFEM [r]) ---> PCFEM [s] :=
    fun r s => Build_RModule_Hom (PCFApp_s r s).
 
@@ -218,4 +256,4 @@ RModule_Hom_struct
 Definition PCFbottom t : Term ---> PCFEM [t] :=
  Build_RModule_Hom (PCFbottom_s t).
 
-
+End close_notation.
